verified/ARMspartan.dfy
@@ -15,21 +15,21 @@ type sp_state = state
 // Spartan-Verification Interface
 //-----------------------------------------------------------------------------
 function sp_eval_op(s:state, o:operand):int
-    requires ValidOperand(s, o);
+    requires ValidState(s)
+    requires ValidOperand(o) || ValidSpecialOperand(s, o)
     { OperandContents(s, o) }
 
 predicate sp_eq_ops(s1:sp_state, s2:sp_state, o:operand)
 {
-    ValidOperand(s1, o)
-        && ValidOperand(s2, o)
+    ValidState(s1) && ValidState(s2) && ValidOperand(o)
         && sp_eval_op(s1, o) == sp_eval_op(s2, o)
 }
 
 function sp_eval_mem(s:state, m:mem):int
-    requires ValidState(s);
-    requires ValidMem(s, m);
+    requires ValidMemState(s.m);
+    requires ValidMem(s.m, m);
     ensures isUInt32(sp_eval_mem(s,m));
-    { MemContents(s, m) }
+    { MemContents(s.m, m) }
 
 function method sp_CNil():codes { CNil }
 function sp_cHead(b:codes):code requires b.sp_CCons? { b.hd }
@@ -62,7 +62,7 @@ function method sp_get_whileBody(c:code):code requires c.While? { c.whileBody }
 //-----------------------------------------------------------------------------
 // This code is pretty much only used for stack-test
 // function method stack(slot:int):operand { OMem(LocalVar(slot)) }
-// function stackval(s:sp_state, o:operand):int requires ValidOperand(s, o); { sp_eval_op(s, o) }
+// function stackval(s:sp_state, o:operand):int requires ValidOperand(o); { sp_eval_op(s, o) }
 // predicate NonEmptyStack(s:sp_state) { s.stack != [] }
 // predicate StackContains(s:sp_state, slot:int) 
 //     requires NonEmptyStack(s);
@@ -79,12 +79,53 @@ function method sp_get_whileBody(c:code):code requires c.While? { c.whileBody }
 //-----------------------------------------------------------------------------
 // Address Helper Functions
 //-----------------------------------------------------------------------------
-function addrval(s:sp_state, a:int):int
+function addrval(s:state, a:int):int
     requires ValidState(s)
-    requires ValidMem(s, Address(a))
+    requires ValidMem(s.m, a)
     ensures isUInt32(addrval(s, a))
 {
-    MemContents(s, Address(a))
+    MemContents(s.m, a)
+}
+
+//-----------------------------------------------------------------------------
+// Useful invariants preserved by instructions
+//-----------------------------------------------------------------------------
+predicate AlwaysInvariant(s:state, s':state)
+{
+    // valid state is maintained
+    ValidState(s) && ValidState(s')
+    // mem validity never changes
+    && (forall m:mem :: m in s.m.addresses <==> m in s'.m.addresses)
+}
+
+predicate ModeInvariant(s:state, s':state)
+    requires ValidState(s) && ValidState(s')
+{
+    mode_of_state(s) == mode_of_state(s')
+}
+
+predicate WorldInvariant(s:state, s':state)
+    requires ValidState(s) && ValidState(s')
+{
+    world_of_state(s) == world_of_state(s')
+}
+
+predicate AllMemInvariant(s:state, s':state)
+    requires ValidState(s) && ValidState(s')
+{
+    s.m == s'.m
+}
+
+predicate GlobalsInvariant(s:state, s':state)
+    requires ValidState(s) && ValidState(s')
+{
+    s.m.globals == s'.m.globals
+}
+
+predicate AddrMemInvariant(s:state, s':state)
+    requires ValidState(s) && ValidState(s')
+{
+    s.m.addresses == s'.m.addresses
 }
 
 //-----------------------------------------------------------------------------
@@ -138,8 +179,8 @@ function method{:opaque} sp_code_STR(rd:operand, base:operand, ofs:operand):code
 function method{:opaque} sp_code_STRglobal(rd:operand, global:operand, base:operand, ofs:operand):code
     { Ins(STR_global(rd, global, base, ofs)) }
 
-function method{:opaque} sp_code_CPS(mod:operand):code
-    { Ins(CPS(mod)) }
+// function method{:opaque} sp_code_CPS(mod:operand):code
+//     { Ins(CPS(mod)) }
 
 function method{:opaque} sp_code_MRS(dst:operand, src:operand):code
     { Ins(MRS(dst, src)) }
@@ -157,10 +198,7 @@ function method{:opaque} sp_code_MOVS():code
     { Ins(MOVS()) }
 
 // Pseudoinstructions  
-function method{:opaque} sp_code_incr(o:operand):code { Ins(ADD(o, o, OConst(1))) }
 function method{:opaque} sp_code_plusEquals(o1:operand, o2:operand):code { Ins(ADD(o1, o1, o2)) }
-function method{:opaque} sp_code_andEquals(o1:operand, o2:operand):code { Ins(AND(o1, o1, o2)) }
-function method{:opaque} sp_code_xorEquals(o1:operand, o2:operand):code { Ins(EOR(o1, o1, o2)) }
 // function method{:opaque} sp_code_push(o:operand):code { 
 //     // Ins(SUB(OSP, OSP, OConst(4)))
 //     var i1 := Ins(SUB(OSP, OSP, OConst(4)));
@@ -177,14 +215,17 @@ function method{:opaque} sp_code_LDRglobaladdr(rd:operand, g:operand):code
 lemma sp_lemma_ADD(s:state, r:state, ok:bool,
     dst:operand, src1:operand, src2:operand)
     requires ValidState(s);
-    requires ValidOperand(s,src1);
-    requires ValidOperand(s,src2);
-    requires ValidDestinationOperand(s, dst);
+    requires ValidOperand(src1);
+    requires ValidOperand(src2);
+    requires ValidDestinationOperand(dst);
     requires isUInt32(OperandContents(s, src1) + OperandContents(s, src2));
     requires sp_eval(sp_code_ADD(dst, src1, src2), s, r, ok);
     ensures  evalUpdate(s, dst, OperandContents(s, src1) +
         OperandContents(s, src2), r, ok);
-    ensures  isUInt32(OperandContents(r, dst));
+    ensures ok;
+    ensures AlwaysInvariant(s, r);
+    ensures AllMemInvariant(s, r);
+    ensures ModeInvariant(s, r);
 {
     reveal_sp_eval();
     reveal_sp_code_ADD();
@@ -193,14 +234,17 @@ lemma sp_lemma_ADD(s:state, r:state, ok:bool,
 lemma sp_lemma_SUB(s:state, r:state, ok:bool,
     dst:operand, src1:operand, src2:operand)
     requires ValidState(s);
-    requires ValidOperand(s,src1);
-    requires ValidOperand(s,src2);
-    requires ValidDestinationOperand(s, dst);
+    requires ValidOperand(src1);
+    requires ValidOperand(src2);
+    requires ValidDestinationOperand(dst);
     requires sp_eval(sp_code_SUB(dst, src1, src2), s, r, ok);
     requires isUInt32(OperandContents(s, src1) - OperandContents(s, src2));
     ensures  evalUpdate(s, dst, OperandContents(s, src1) -
         OperandContents(s, src2), r, ok);
-    ensures  isUInt32(OperandContents(r, dst));
+    ensures ok;
+    ensures AlwaysInvariant(s, r);
+    ensures AllMemInvariant(s, r);
+    ensures ModeInvariant(s, r);
 {
     reveal_sp_eval();
     reveal_sp_code_SUB();
@@ -209,14 +253,17 @@ lemma sp_lemma_SUB(s:state, r:state, ok:bool,
 lemma sp_lemma_MUL(s:state, r:state, ok:bool,
     dst:operand, src1:operand, src2:operand)
     requires ValidState(s);
-    requires ValidRegOperand(s,src1);
-    requires ValidRegOperand(s,src2);
-    requires ValidDestinationOperand(s, dst);
+    requires ValidRegOperand(src1);
+    requires ValidRegOperand(src2);
+    requires ValidDestinationOperand(dst);
     requires sp_eval(sp_code_MUL(dst, src1, src2), s, r, ok);
     requires isUInt32(OperandContents(s, src1) * OperandContents(s, src2));
     ensures  evalUpdate(s, dst, OperandContents(s, src1) *
         OperandContents(s, src2), r, ok);
-    ensures  isUInt32(OperandContents(r, dst));
+    ensures ok;
+    ensures AlwaysInvariant(s, r);
+    ensures AllMemInvariant(s, r);
+    ensures ModeInvariant(s, r);
 {
     reveal_sp_eval();
     reveal_sp_code_MUL();
@@ -225,15 +272,18 @@ lemma sp_lemma_MUL(s:state, r:state, ok:bool,
 lemma sp_lemma_UDIV(s:state, r:state, ok:bool,
     dst:operand, src1:operand, src2:operand)
     requires ValidState(s);
-    requires ValidOperand(s,src1);
-    requires ValidOperand(s,src2);
-    requires ValidDestinationOperand(s, dst);
+    requires ValidOperand(src1);
+    requires ValidOperand(src2);
+    requires ValidDestinationOperand(dst);
     requires OperandContents(s,src2) > 0;
     requires sp_eval(sp_code_UDIV(dst, src1, src2), s, r, ok);
     requires isUInt32(OperandContents(s, src1) / OperandContents(s, src2));
     ensures  evalUpdate(s, dst, OperandContents(s, src1) /
         OperandContents(s, src2), r, ok);
-    ensures  isUInt32(OperandContents(r, dst));
+    ensures ok;
+    ensures AlwaysInvariant(s, r);
+    ensures AllMemInvariant(s, r);
+    ensures ModeInvariant(s, r);
 {
     reveal_sp_eval();
     reveal_sp_code_UDIV();
@@ -242,13 +292,16 @@ lemma sp_lemma_UDIV(s:state, r:state, ok:bool,
 lemma sp_lemma_AND(s:state, r:state, ok:bool,
     dst:operand, src1:operand, src2:operand)
     requires ValidState(s);
-    requires ValidOperand(s,src1);
-    requires ValidOperand(s,src2);
-    requires ValidDestinationOperand(s, dst);
+    requires ValidOperand(src1);
+    requires ValidOperand(src2);
+    requires ValidDestinationOperand(dst);
     requires sp_eval(sp_code_AND(dst, src1, src2), s, r, ok);
     ensures evalUpdate(s, dst, and32(eval_op(s, src1),
         eval_op(s, src2)), r, ok);
-    ensures  isUInt32(OperandContents(r, dst));
+    ensures ok;
+    ensures AlwaysInvariant(s, r);
+    ensures AllMemInvariant(s, r);
+    ensures ModeInvariant(s, r);
 {
     reveal_sp_eval();
     reveal_sp_code_AND();
@@ -257,13 +310,16 @@ lemma sp_lemma_AND(s:state, r:state, ok:bool,
 lemma sp_lemma_ORR(s:state, r:state, ok:bool,
     dst:operand, src1:operand, src2:operand)
     requires ValidState(s);
-    requires ValidOperand(s,src1);
-    requires ValidOperand(s,src2);
-    requires ValidDestinationOperand(s, dst);
+    requires ValidOperand(src1);
+    requires ValidOperand(src2);
+    requires ValidDestinationOperand(dst);
     requires sp_eval(sp_code_ORR(dst, src1, src2), s, r, ok);
     ensures evalUpdate(s, dst, or32(eval_op(s, src1),
         eval_op(s, src2)), r, ok);
-    ensures  isUInt32(OperandContents(r, dst));
+    ensures ok;
+    ensures AlwaysInvariant(s, r);
+    ensures AllMemInvariant(s, r);
+    ensures ModeInvariant(s, r);
 {
     reveal_sp_eval();
     reveal_sp_code_ORR();
@@ -272,13 +328,16 @@ lemma sp_lemma_ORR(s:state, r:state, ok:bool,
 lemma sp_lemma_EOR(s:state, r:state, ok:bool,
     dst:operand, src1:operand, src2:operand)
     requires ValidState(s);
-    requires ValidOperand(s,src1);
-    requires ValidOperand(s,src2);
-    requires ValidDestinationOperand(s, dst);
+    requires ValidOperand(src1);
+    requires ValidOperand(src2);
+    requires ValidDestinationOperand(dst);
     requires sp_eval(sp_code_EOR(dst, src1, src2), s, r, ok);
     ensures evalUpdate(s, dst, xor32(eval_op(s, src1),
         eval_op(s, src2)), r, ok);
-    ensures  isUInt32(OperandContents(r, dst));
+    ensures ok;
+    ensures AlwaysInvariant(s, r);
+    ensures AllMemInvariant(s, r);
+    ensures ModeInvariant(s, r);
 {
     reveal_sp_eval();
     reveal_sp_code_EOR();
@@ -287,14 +346,17 @@ lemma sp_lemma_EOR(s:state, r:state, ok:bool,
 lemma sp_lemma_ROR(s:state, r:state, ok:bool,
     dst:operand, src1:operand, src2:operand)
     requires ValidState(s);
-    requires ValidOperand(s,src1);
+    requires ValidOperand(src1);
     requires ValidShiftOperand(s,src2);
-    requires ValidDestinationOperand(s, dst);
+    requires ValidDestinationOperand(dst);
     requires sp_eval(sp_code_ROR(dst, src1, src2), s, r, ok);
     requires src2.OConst?;
     ensures evalUpdate(s, dst, ror32(eval_op(s, src1),
         eval_op(s, src2)), r, ok);
-    ensures  isUInt32(OperandContents(r, dst));
+    ensures ok;
+    ensures AlwaysInvariant(s, r);
+    ensures AllMemInvariant(s, r);
+    ensures ModeInvariant(s, r);
 {
     reveal_sp_eval();
     reveal_sp_code_ROR();
@@ -303,14 +365,17 @@ lemma sp_lemma_ROR(s:state, r:state, ok:bool,
 lemma sp_lemma_LSL(s:state, r:state, ok:bool,
     dst:operand, src1:operand, src2:operand)
     requires ValidState(s);
-    requires ValidOperand(s,src1);
+    requires ValidOperand(src1);
     requires ValidShiftOperand(s,src2);
-    requires ValidDestinationOperand(s, dst);
+    requires ValidDestinationOperand(dst);
     requires sp_eval(sp_code_LSL(dst, src1, src2), s, r, ok);
     requires src2.OConst?;
     ensures evalUpdate(s, dst, shl32(eval_op(s, src1),
         eval_op(s, src2)), r, ok);
-    ensures  isUInt32(OperandContents(r, dst));
+    ensures ok;
+    ensures AlwaysInvariant(s, r);
+    ensures AllMemInvariant(s, r);
+    ensures ModeInvariant(s, r);
 {
     reveal_sp_eval();
     reveal_sp_code_LSL();
@@ -319,14 +384,17 @@ lemma sp_lemma_LSL(s:state, r:state, ok:bool,
 lemma sp_lemma_LSR(s:state, r:state, ok:bool,
     dst:operand, src1:operand, src2:operand)
     requires ValidState(s);
-    requires ValidOperand(s,src1);
+    requires ValidOperand(src1);
     requires ValidShiftOperand(s,src2);
-    requires ValidDestinationOperand(s, dst);
+    requires ValidDestinationOperand(dst);
     requires sp_eval(sp_code_LSR(dst, src1, src2), s, r, ok);
     requires src2.OConst?;
     ensures evalUpdate(s, dst, shr32(eval_op(s, src1),
         eval_op(s, src2)), r, ok);
-    ensures  isUInt32(OperandContents(r, dst));
+    ensures ok;
+    ensures AlwaysInvariant(s, r);
+    ensures AllMemInvariant(s, r);
+    ensures ModeInvariant(s, r);
 {
     reveal_sp_eval();
     reveal_sp_code_LSR();
@@ -335,12 +403,15 @@ lemma sp_lemma_LSR(s:state, r:state, ok:bool,
 lemma sp_lemma_MVN(s:state, r:state, ok:bool,
     dst:operand, src:operand)
     requires ValidState(s);
-    requires ValidOperand(s,src);
-    requires ValidDestinationOperand(s, dst);
+    requires ValidOperand(src);
+    requires ValidDestinationOperand(dst);
     requires sp_eval(sp_code_MVN(dst, src), s, r, ok);
     ensures evalUpdate(s, dst, not32(eval_op(s, src)),
         r, ok);
-    ensures  isUInt32(OperandContents(r, dst));
+    ensures ok;
+    ensures AlwaysInvariant(s, r);
+    ensures AllMemInvariant(s, r);
+    ensures ModeInvariant(s, r);
 {
     reveal_sp_eval();
     reveal_sp_code_MVN();
@@ -349,11 +420,14 @@ lemma sp_lemma_MVN(s:state, r:state, ok:bool,
 lemma sp_lemma_MOV(s:state, r:state, ok:bool,
     dst:operand, src:operand)
     requires ValidState(s);
-    requires ValidOperand(s, src);
-    requires ValidDestinationOperand(s, dst);
+    requires ValidOperand(src);
+    requires ValidDestinationOperand(dst);
     requires sp_eval(sp_code_MOV(dst, src), s, r, ok);
     ensures evalUpdate(s, dst, OperandContents(s, src), r, ok);
-    ensures isUInt32(OperandContents(r, dst));
+    ensures ok;
+    ensures AlwaysInvariant(s, r);
+    ensures AllMemInvariant(s, r);
+    ensures ModeInvariant(s, r);
 {
     reveal_sp_eval();
     reveal_sp_code_MOV();
@@ -362,14 +436,17 @@ lemma sp_lemma_MOV(s:state, r:state, ok:bool,
 lemma sp_lemma_LDR(s:state, r:state, ok:bool,
     rd:operand, base:operand, ofs:operand)
     requires ValidState(s);
-    requires ValidDestinationOperand(s, rd);
-    requires ValidOperand(s, base);
-    requires ValidOperand(s, ofs);
+    requires ValidDestinationOperand(rd);
+    requires ValidOperand(base);
+    requires ValidOperand(ofs);
     requires WordAligned(OperandContents(s, base) + OperandContents(s, ofs));
-    requires ValidMem(s, addr_mem(s, base, ofs));
+    requires ValidMem(s.m, addr_mem(s, base, ofs));
     requires sp_eval(sp_code_LDR(rd, base, ofs), s, r, ok);
-    ensures evalUpdate(s, rd, MemContents(s, Address(OperandContents(s, base) + OperandContents(s, ofs))), r, ok)
-    ensures isUInt32(OperandContents(r, rd));
+    ensures evalUpdate(s, rd, MemContents(s.m, OperandContents(s, base) + OperandContents(s, ofs)), r, ok)
+    ensures ok;
+    ensures AlwaysInvariant(s, r);
+    ensures AllMemInvariant(s, r);
+    ensures ModeInvariant(s, r);
 {
     reveal_sp_eval();
     reveal_sp_code_LDR();
@@ -378,15 +455,17 @@ lemma sp_lemma_LDR(s:state, r:state, ok:bool,
 lemma sp_lemma_LDRglobal(s:state, r:state, ok:bool,
     rd:operand, g:operand, base:operand, ofs:operand)
     requires ValidState(s);
-    requires ValidDestinationOperand(s, rd);
-    requires ValidOperand(s, base);
-    requires ValidOperand(s, ofs);
-    requires ValidGlobalState(s);
+    requires ValidDestinationOperand(rd);
+    requires ValidOperand(base);
+    requires ValidOperand(ofs);
     requires ValidGlobalOffset(g, OperandContents(s, ofs));
     requires AddressOfGlobal(g) == OperandContents(s, base);
     requires sp_eval(sp_code_LDRglobal(rd, g, base, ofs), s, r, ok);
-    ensures evalUpdate(s, rd, GlobalWord(s, g, OperandContents(s, ofs)), r, ok);
-    ensures isUInt32(OperandContents(r, rd));
+    ensures evalUpdate(s, rd, GlobalWord(s.m, g, OperandContents(s, ofs)), r, ok);
+    ensures ok;
+    ensures AlwaysInvariant(s, r);
+    ensures AllMemInvariant(s, r);
+    ensures ModeInvariant(s, r);
 {
     reveal_sp_eval();
     reveal_sp_code_LDRglobal();
@@ -395,15 +474,18 @@ lemma sp_lemma_LDRglobal(s:state, r:state, ok:bool,
 lemma sp_lemma_STR(s:state, r:state, ok:bool,
     rd:operand, base:operand, ofs:operand)
     requires ValidState(s);
-    requires ValidRegOperand(s, rd);
-    requires ValidOperand(s, base);
-    requires ValidOperand(s, ofs);
+    requires ValidRegOperand(rd);
+    requires ValidOperand(base);
+    requires ValidOperand(ofs);
     requires WordAligned(OperandContents(s, base) + OperandContents(s, ofs));
-    requires ValidMem(s, addr_mem(s, base, ofs));
+    requires ValidMem(s.m, addr_mem(s, base, ofs));
     requires sp_eval(sp_code_STR(rd, base, ofs), s, r, ok);
-    ensures evalMemUpdate(s, Address(OperandContents(s, base) + OperandContents(s, ofs)),
+    ensures evalMemUpdate(s, OperandContents(s, base) + OperandContents(s, ofs),
         OperandContents(s, rd), r, ok)
-    ensures ValidMem(r, addr_mem(s, base, ofs));
+    ensures ok;
+    ensures AlwaysInvariant(s, r);
+    ensures GlobalsInvariant(s, r);
+    ensures ModeInvariant(s, r);
 {
     reveal_sp_eval();
     reveal_sp_code_STR();
@@ -412,37 +494,43 @@ lemma sp_lemma_STR(s:state, r:state, ok:bool,
 lemma sp_lemma_STRglobal(s:state, r:state, ok:bool,
     rd:operand, g:operand, base:operand, ofs:operand)
     requires ValidState(s);
-    requires ValidRegOperand(s, rd);
-    requires ValidOperand(s, base);
-    requires ValidOperand(s, ofs);
-    requires ValidGlobalState(s);
+    requires ValidRegOperand(rd);
+    requires ValidOperand(base);
+    requires ValidOperand(ofs);
     requires ValidGlobalOffset(g, OperandContents(s, ofs));
     requires AddressOfGlobal(g) == OperandContents(s, base);
     requires sp_eval(sp_code_STRglobal(rd, g, base, ofs), s, r, ok);
     ensures evalGlobalUpdate(s, g, OperandContents(s, ofs), OperandContents(s, rd), r, ok);
+    ensures ok;
+    ensures AlwaysInvariant(s, r);
+    ensures ModeInvariant(s, r);
+    ensures AddrMemInvariant(s, r);
 {
     reveal_sp_eval();
     reveal_sp_code_STRglobal();
 }
 
-lemma sp_lemma_CPS(s:state, r:state, ok:bool, mod:operand)
-    requires ValidState(s);
-    requires ValidOperand(s, mod);
-    requires sp_eval(sp_code_CPS(mod), s, r, ok);
-    requires ValidModeEncoding(OperandContents(s, mod));
-    ensures  evalModeUpdate(s, OperandContents(s, mod), r, ok);
-{
-    reveal_sp_eval();
-    reveal_sp_code_CPS();
-}
+// lemma sp_lemma_CPS(s:state, r:state, ok:bool, mod:operand)
+//     requires ValidState(s);
+//     requires ValidOperand(mod);
+//     requires sp_eval(sp_code_CPS(mod), s, r, ok);
+//     requires ValidModeEncoding(OperandContents(s, mod));
+//     ensures  evalModeUpdate(s, OperandContents(s, mod), r, ok);
+//     ensures ok;
+//     ensures AlwaysInvariant(s, r);
+//     ensures AllMemInvariant(s, r);
+// {
+//     reveal_sp_eval();
+//     reveal_sp_code_CPS();
+// }
 
 lemma sp_lemma_MRS(s:state, r:state, ok:bool,
     dst:operand, src: operand)
     requires ValidState(s)
     requires ValidSpecialOperand(s, src)
-    requires ValidRegOperand(s, dst)
+    requires ValidRegOperand(dst)
     requires sp_eval(sp_code_MRS(dst, src), s, r, ok)
-    requires evalUpdate(s, dst, OperandContents(s, src), r, ok)
+    ensures evalUpdate(s, dst, OperandContents(s, src), r, ok)
 {
     reveal_sp_eval();
     reveal_sp_code_MRS();
@@ -451,8 +539,10 @@ lemma sp_lemma_MRS(s:state, r:state, ok:bool,
 lemma sp_lemma_MSR(s:state, r:state, ok:bool,
     dst:operand, src: operand)
     requires ValidState(s)
-    requires ValidRegOperand(s, src)
+    requires ValidRegOperand(src)
     requires ValidSpecialOperand(s, dst)
+    requires dst.OSReg? && dst.sr.cpsr? ==>
+        ValidModeEncoding(and32(OperandContents(s, src), 0x1f))
     requires sp_eval(sp_code_MSR(dst, src), s, r, ok)
     ensures evalSRegUpdate(s, dst, OperandContents(s, src), r, ok)
 {
@@ -462,10 +552,10 @@ lemma sp_lemma_MSR(s:state, r:state, ok:bool,
 
 lemma sp_lemma_MRC(s:state, r:state, ok:bool, dst:operand)
     requires ValidState(s);
-    requires ValidRegOperand(s, dst);
+    requires ValidRegOperand(dst);
     requires ValidSCR(s);
     requires sp_eval(sp_code_MRC(dst), s, r, ok);
-    ensures  evalUpdate(s, dst, s.sregs[scr], r, ok);
+    ensures  evalUpdate(s, dst, SCRContents(s), r, ok);
 {
     reveal_sp_eval();
     reveal_sp_code_MRC();
@@ -473,7 +563,7 @@ lemma sp_lemma_MRC(s:state, r:state, ok:bool, dst:operand)
 
 lemma sp_lemma_MCR(s:state, r:state, ok:bool, src:operand)
     requires ValidState(s)
-    requires ValidRegOperand(s, src)
+    requires ValidRegOperand(src)
 	requires ValidSCR(s)
     requires sp_eval(sp_code_MCR(src), s, r, ok)
     ensures  evalSRegUpdate(s, OSReg(scr), OperandContents(s,src), r, ok)
@@ -486,27 +576,28 @@ lemma sp_lemma_MOVS(s:state, r:state, ok:bool)
     requires ValidState(s)
     requires !(mode_of_state(s) == User)
     requires sp_eval(sp_code_MOVS(), s, r, ok)
-    ensures evalSRegUpdate(s, OSReg(cpsr), s.sregs[scr], r, ok)
+    requires ValidModeEncoding(and32(OperandContents(s, OSPSR), 0x1f))
+    ensures  evalSRegUpdate(s, OSReg(cpsr), OperandContents(s,OSPSR), r, ok)
 {
     reveal_sp_eval();
     reveal_sp_code_MOVS();
 }
 
 // Lemmas for frontend functions
-lemma sp_lemma_incr(s:sp_state, r:sp_state, ok:bool, o:operand)
-    requires ValidState(s);
-    requires ValidDestinationOperand(s, o)
-    requires sp_eval(sp_code_incr(o), s, r, ok)
-    requires isUInt32(eval_op(s, o) + 1);
-    ensures  evalUpdate(s, o, OperandContents(s, o) + 1, r, ok)
-{
-    reveal_sp_eval();
-    reveal_sp_code_incr();
-}
+// lemma sp_lemma_incr(s:sp_state, r:sp_state, ok:bool, o:operand)
+//     requires ValidState(s);
+//     requires ValidDestinationOperand(o)
+//     requires sp_eval(sp_code_incr(o), s, r, ok)
+//     requires isUInt32(eval_op(s, o) + 1);
+//     ensures  evalUpdate(s, o, OperandContents(s, o) + 1, r, ok)
+// {
+//     reveal_sp_eval();
+//     reveal_sp_code_incr();
+// }
 
 // lemma sp_lemma_push(s:sp_state, r:sp_state, ok:bool, o:operand)
-//     requires ValidDestinationOperand(s, OSP)
-//     requires ValidOperand(s, o)
+//     requires ValidDestinationOperand(OSP)
+//     requires ValidOperand(o)
 //     requires sp_eval(sp_code_push(o), s, r, ok)
 //     requires 4 <= eval_op(s, o) < MaxVal()
 //     requires ValidMem(s, Address(eval_op(s, OSP)))
@@ -523,47 +614,31 @@ lemma sp_lemma_incr(s:sp_state, r:sp_state, ok:bool, o:operand)
 
 lemma sp_lemma_plusEquals(s:sp_state, r:sp_state, ok:bool, o1:operand, o2:operand)
     requires ValidState(s);
-    requires ValidDestinationOperand(s, o1);
-    requires ValidOperand(s, o2);
+    requires ValidDestinationOperand(o1);
+    requires ValidOperand(o2);
     requires sp_eval(sp_code_plusEquals(o1, o2), s, r, ok);
     requires isUInt32(OperandContents(s, o1) + OperandContents(s, o2));
     ensures evalUpdate(s, o1, OperandContents(s, o1) +
         OperandContents(s, o2), r, ok);
+    ensures ok;
+    ensures AlwaysInvariant(s, r);
+    ensures AllMemInvariant(s, r);
+    ensures ModeInvariant(s, r);
 {
     reveal_sp_eval();
     reveal_sp_code_plusEquals();
 }
 
-lemma sp_lemma_andEquals(s:sp_state, r:sp_state, ok:bool, o1:operand, o2:operand)
-    requires ValidState(s);
-    requires ValidDestinationOperand(s, o1);
-    requires ValidOperand(s, o2);
-    requires sp_eval(sp_code_andEquals(o1, o2), s, r, ok);
-    ensures evalUpdate(s, o1, and32(eval_op(s, o1), eval_op(s, o2)), r, ok);
-{
-    reveal_sp_eval();
-    reveal_sp_code_andEquals();
-}
-
-lemma sp_lemma_xorEquals(s:sp_state, r:sp_state, ok:bool, o1:operand, o2:operand)
-    requires ValidState(s);
-    requires ValidDestinationOperand(s, o1);
-    requires ValidOperand(s, o2);
-    requires sp_eval(sp_code_xorEquals(o1, o2), s, r, ok);
-    ensures evalUpdate(s, o1, xor32(eval_op(s, o1), eval_op(s, o2)), r, ok);
-{
-    reveal_sp_eval();
-    reveal_sp_code_xorEquals();
-}
-
 lemma sp_lemma_LDRglobaladdr(s:state, r:state, ok:bool, rd:operand, g:operand)
     requires ValidState(s);
-    requires ValidDestinationOperand(s, rd);
+    requires ValidDestinationOperand(rd);
     requires ValidGlobal(g);
     requires sp_eval(sp_code_LDRglobaladdr(rd, g), s, r, ok);
     ensures evalUpdate(s, rd, AddressOfGlobal(g), r, ok);
-    ensures isUInt32(OperandContents(r, rd));
-    ensures AddressOfGlobal(g) == OperandContents(r, rd);
+    ensures ok;
+    ensures AlwaysInvariant(s, r);
+    ensures AllMemInvariant(s, r);
+    ensures ModeInvariant(s, r);
 {
     reveal_sp_eval();
     reveal_sp_code_LDRglobaladdr();
@@ -597,8 +672,9 @@ lemma sp_lemma_block(b:codes, s0:state, r:state, ok:bool) returns(r1:state, ok1:
 }
 
 lemma sp_lemma_ifElse(ifb:obool, ct:code, cf:code, s:state, r:state, ok:bool) returns(cond:bool)
-  requires ValidOperand(s, ifb.o1);
-  requires ValidOperand(s, ifb.o2);
+  requires ValidState(s);
+  requires ValidOperand(ifb.o1);
+  requires ValidOperand(ifb.o2);
   requires sp_eval(IfElse(ifb, ct, cf), s, r, ok)
   ensures  cond == evalOBool(s, ifb)
   ensures  (if cond then sp_eval(ct, s, r, ok) else sp_eval(cf, s, r, ok))
@@ -622,8 +698,8 @@ predicate sp_whileInv(b:obool, c:code, n:int, r1:state, ok1:bool, r2:state, ok2:
 }
 
 lemma sp_lemma_while(b:obool, c:code, s:state, r:state, ok:bool) returns(n:nat, r':state, ok':bool)
-  requires ValidOperand(s, b.o1)
-  requires ValidOperand(s, b.o2)
+  requires ValidOperand(b.o1)
+  requires ValidOperand(b.o2)
   requires sp_eval(While(b, c), s, r, ok)
   ensures  evalWhileOpaque(b, c, n, s, r, ok)
   ensures  ok'
@@ -638,8 +714,9 @@ lemma sp_lemma_while(b:obool, c:code, s:state, r:state, ok:bool) returns(n:nat, 
 }
 
 lemma sp_lemma_whileTrue(b:obool, c:code, n:nat, s:state, r:state, ok:bool) returns(r':state, ok':bool)
-  requires ValidOperand(s, b.o1)
-  requires ValidOperand(s, b.o2)
+  requires ValidState(s)
+  requires ValidOperand(b.o1)
+  requires ValidOperand(b.o2)
   requires n > 0
   requires evalWhileOpaque(b, c, n, s, r, ok)
   ensures  evalOBool(s, b)
@@ -652,8 +729,9 @@ lemma sp_lemma_whileTrue(b:obool, c:code, n:nat, s:state, r:state, ok:bool) retu
 }
 
 lemma sp_lemma_whileFalse(b:obool, c:code, s:state, r:state, ok:bool)
-  requires ValidOperand(s, b.o1)
-  requires ValidOperand(s, b.o2)
+  requires ValidState(s)
+  requires ValidOperand(b.o1)
+  requires ValidOperand(b.o2)
   requires evalWhileOpaque(b, c, 0, s, r, ok)
   ensures  !evalOBool(s, b)
   ensures  ok
